isabelle/Core/SmallStepF.thy
@@ -1,0 +1,630 @@
+theory SmallStepF
+imports Main Util.MList Util.SList ListTools Semantics "HOL-Library.Product_Lexorder" "HOL.Product_Type" "HOL-IMP.Star"
+begin
+
+type_synonym Configuration = "Contract * State * Environment * (ReduceWarning list) * (Payment list)"
+
+inductive
+  small_step_reduce :: "Configuration \<Rightarrow> Configuration \<Rightarrow> bool" (infix "\<rightarrow>" 55)
+where
+CloseRefund:  "refundOne (accounts s) = Some ((party, token, money), newAccount) \<Longrightarrow>
+  (Close, s, env, warns, payments) \<rightarrow>
+  (Close, (s\<lparr>accounts := newAccount\<rparr>), env, warns @ [ReduceNoWarning], payments @ [Payment party (Party party) token money])" |
+PayNonPositive: "evalValue env s val \<le> 0 \<Longrightarrow>
+  (Pay accId payee token val cont, s, env, warns, payments) \<rightarrow>
+  (cont, s, env, warns @ [ReduceNonPositivePay accId payee token (evalValue env s val)], payments)" |
+PayPositivePartialWithPayment: "\<lbrakk>evalValue env s val > 0;
+  evalValue env s val > moneyInAccount accId token (accounts s);
+  updateMoneyInAccount accId token 0 (accounts s) = newAccs;
+  moneyInAccount accId token (accounts s) = moneyToPay;
+  giveMoney accId payee token (moneyToPay) newAccs = (payment, finalAccs);
+  payment = ReduceWithPayment somePayment\<rbrakk> \<Longrightarrow>
+  (Pay accId payee token val cont, s, env, warns, payments) \<rightarrow>
+  ((cont, s\<lparr>accounts := finalAccs\<rparr>, env, warns @ [ReducePartialPay accId payee token moneyToPay (evalValue env s val)], payments @ [somePayment]))" |
+PayPositivePartialWithoutPayment: "\<lbrakk>evalValue env s val > 0;
+  evalValue env s val > moneyInAccount accId token (accounts s);
+  updateMoneyInAccount accId token 0 (accounts s) = newAccs;
+  moneyInAccount accId token (accounts s) = moneyToPay;
+  giveMoney accId payee token (moneyToPay) newAccs = (payment, finalAccs);
+  payment = ReduceNoPayment\<rbrakk> \<Longrightarrow>
+  (Pay accId payee token val cont, s, env, warns, payments) \<rightarrow>
+  ((cont, s\<lparr>accounts := finalAccs\<rparr>, env, warns @ [ReducePartialPay accId payee token moneyToPay (evalValue env s val)], payments))" |
+PayPositiveFullWithPayment: "\<lbrakk>evalValue env s val > 0;
+  evalValue env s val \<le> moneyInAccount accId token (accounts s);
+  moneyInAccount accId token (accounts s) = moneyInAcc;
+  moneyInAcc - (evalValue env s val) = newBalance;
+  updateMoneyInAccount accId token newBalance (accounts s) = newAccs;
+  giveMoney accId payee token (evalValue env s val) newAccs = (payment, finalAccs);
+  payment = ReduceWithPayment somePayment\<rbrakk> \<Longrightarrow>
+  (Pay accId payee token val cont, s, env, warns, payments) \<rightarrow>
+  (cont, s\<lparr>accounts := finalAccs\<rparr>, env, warns @ [ReduceNoWarning], payments @ [somePayment])" |
+PayPositiveFullWithoutPayment: "\<lbrakk>evalValue env s val > 0;
+  evalValue env s val \<le> moneyInAccount accId token (accounts s);
+  moneyInAccount accId token (accounts s) = moneyInAcc;
+  moneyInAcc - (evalValue env s val) = newBalance;
+  updateMoneyInAccount accId token newBalance (accounts s) = newAccs;
+  giveMoney accId payee token (evalValue env s val) newAccs = (payment, finalAccs);
+  payment = ReduceNoPayment\<rbrakk> \<Longrightarrow>
+  (Pay accId payee token val cont, s, env, warns, payments) \<rightarrow>
+  (cont, s\<lparr>accounts := finalAccs\<rparr>, env, warns @ [ReduceNoWarning], payments)"  |
+IfTrue: "evalObservation env s obs \<Longrightarrow>
+  (If obs cont1 cont2, s, env, warns, payments) \<rightarrow>
+  (cont1, s, env, warns @ [ReduceNoWarning], payments)" |
+IfFalse: "\<not>evalObservation env s obs \<Longrightarrow>
+  (If obs cont1 cont2, s, env, warns, payments) \<rightarrow>
+  (cont2, s, env, warns @ [ReduceNoWarning], payments)" |
+WhenTimeout: "\<lbrakk>slotInterval env = (startSlot, endSlot);
+  endSlot \<ge> timeout;
+  startSlot \<ge> timeout\<rbrakk> \<Longrightarrow>
+  (When cases timeout cont, s, env, warns, payments) \<rightarrow>
+  (cont, s, env, warns @ [ReduceNoWarning], payments)"|
+LetShadow: "lookup valId (boundValues s) = Some oldVal \<Longrightarrow>
+  (Let valId val cont, s, env, warns, payments) \<rightarrow>
+  (cont, s\<lparr> boundValues := MList.insert valId (evalValue env s val) (boundValues s)\<rparr>, env, warns @ [ReduceShadowing valId oldVal (evalValue env s val)], payments)" |
+LetNoShadow: "lookup valId (boundValues s) = None \<Longrightarrow>
+  (Let valId val cont, s, env, warns, payments) \<rightarrow>
+  (cont, s\<lparr> boundValues := MList.insert valId (evalValue env s val) (boundValues s)\<rparr>, env, warns @ [ReduceNoWarning], payments)"  |
+AssertTrue: "evalObservation env s obs \<Longrightarrow>
+  (Assert obs cont, s, env, warns, payments) \<rightarrow>
+  (cont, s, env, warns @ [ReduceNoWarning], payments)" |
+AssertFalse: "\<not>evalObservation env s obs \<Longrightarrow>
+  (Assert obs cont, s, env, warns, payments) \<rightarrow>
+  (cont, s, env, warns @ [ReduceAssertionFailed], payments)"
+
+abbreviation
+  small_step_reduces :: "Configuration \<Rightarrow> Configuration \<Rightarrow> bool" (infix "\<rightarrow>*" 55)
+  where "x \<rightarrow>* y == star small_step_reduce x y"
+
+(*Small Step Induction from FaustusSemantics*)
+thm small_step_reduce.induct
+lemmas small_step_reduce_induct = small_step_reduce.induct[split_format(complete)]
+declare small_step_reduce.intros[simp,intro]
+
+(*Needed to use Elimination rules for smallStepReductionImpReduceStep lemma*)
+inductive_cases CloseE[elim]: "(Close, s, env, warns, payments) \<rightarrow> ct"
+thm CloseE
+inductive_cases PayE[elim!]: "(Pay accId payee token val cont, s, env, warns, payments) \<rightarrow> ct"
+thm PayE
+inductive_cases IfE[elim!]: "(If obs cont1 cont2, s, env, warns, payments) \<rightarrow> ct"
+thm IfE
+inductive_cases WhenE[elim!]: "(When cases timeout cont, s, env, warns, payments) \<rightarrow> ct"
+thm WhenE
+inductive_cases LetE[elim!]: "(Let valId val cont, s, env, warns, payments) \<rightarrow> ct"
+thm LetE
+inductive_cases AssertE[elim!]: "(Assert obs cont, s, env, warns, payments) \<rightarrow> ct"
+thm AssertE
+
+(*Warning Lemmas*)
+lemma smallStepWarningsAreArbitrary:
+"(c,  s, e, w, p) \<rightarrow> (c', s', e', w', p') \<Longrightarrow>
+  (\<forall>w'' . \<exists>w''' . (c, s, e, w'', p) \<rightarrow> (c', s', e', w''', p'))"
+proof (induction c s e w p c' s' e' w' p' rule: small_step_reduce_induct)
+  case (CloseRefund s party token money newAccount env warns payments)
+  then show ?case by auto
+next
+  case (PayNonPositive env s val accId payee token cont warns payments)
+  then show ?case by auto
+next
+  case (PayPositivePartialWithPayment env s val accId token newAccs moneyToPay payee payment finalAccs somePayment cont warns payments)
+  then show ?case apply auto
+    apply (cases "lookup (accId, token) (accounts s)", auto)
+    sorry
+(*
+     apply fastforce
+    by fastforce*)
+next
+  case (PayPositivePartialWithoutPayment env s val accId token newAccs moneyToPay payee payment finalAccs cont warns payments)
+  then show ?case apply auto
+    sorry
+    (*apply (cases "lookup (accId, token) (accounts s)", auto)
+     apply fastforce
+    by fastforce*)
+next
+  case (PayPositiveFullWithPayment env s val accId token moneyInAcc newBalance newAccs payee payment finalAccs somePayment cont warns payments)
+  then show ?case apply auto
+    apply (cases "lookup (accId, token) (accounts s)", auto)
+    apply (cases "moneyInAcc = evalValue env s val", auto)
+     apply fastforce
+    by fastforce
+next
+  case (PayPositiveFullWithoutPayment env s val accId token moneyInAcc newBalance newAccs payee payment finalAccs cont warns payments)
+  then show ?case apply auto
+    sorry
+    (*
+    apply (cases "lookup (accId, token) (accounts s)", auto)
+    apply (cases "moneyInAcc = evalValue env s val", auto)
+     apply fastforce
+    by fastforce*)
+next
+  case (IfTrue env s obs cont1 cont2 warns payments)
+  then show ?case by auto
+next
+  case (IfFalse env s obs cont1 cont2 warns payments)
+  then show ?case by auto
+next
+  case (WhenTimeout env startSlot endSlot timeout cases cont s warns payments)
+  then show ?case by auto
+next
+  case (LetShadow valId s oldVal val cont env warns payments)
+  then show ?case by auto
+next
+  case (LetNoShadow valId s val cont env warns payments)
+  then show ?case by auto
+next
+  case (AssertTrue env s obs cont warns payments)
+  then show ?case by auto
+next
+  case (AssertFalse env s obs cont warns payments)
+  then show ?case by auto
+qed
+
+lemma smallStepStarWarningsAreArbitrary:
+  "(c, s, e, w, p) \<rightarrow>* (c', s', e', w'', p') \<Longrightarrow>
+    (\<forall>w'' . \<exists>w''' . (c, s, e, w'', p) \<rightarrow>* (c', s', e', w''', p'))"
+apply (induction rule: star.induct[of "small_step_reduce", split_format(complete)], auto)
+  by (meson smallStepWarningsAreArbitrary star.step)
+
+definition "finalMarlowe cs \<longleftrightarrow> \<not>(\<exists>cs'. cs \<rightarrow> cs')"
+
+lemma finalD:
+"finalMarlowe (contract, s, e, w, p) \<Longrightarrow>
+  contract = Close \<or> (\<exists> cases timeout continue . contract = When cases timeout continue)"
+  apply (auto simp add: finalMarlowe_def)
+  apply (cases contract, auto)
+     apply (meson PayNonPositive PayPositiveFullWithPayment PayPositiveFullWithoutPayment PayPositivePartialWithPayment PayPositivePartialWithoutPayment giveMoney.elims not_less)
+    apply (meson IfFalse IfTrue)
+   apply (meson LetShadow option.exhaust_sel small_step_reduce.intros(11))
+  by (meson small_step_reduce.intros(12) small_step_reduce.intros(13))
+
+(*BEGIN proof of Reduce Step is a Small Step Reduction in Marlowe*)
+lemma reduceStepIsSmallStepReduction:
+assumes "reduceContractStep env state contract = Reduced warning paymentReduceResult newState continueContract"
+shows "\<exists> appendPayment .(contract, state, env, initialWarnings, initialPayments) \<rightarrow> (continueContract, newState, env, initialWarnings @ [warning], initialPayments @ appendPayment)"
+proof (cases contract paymentReduceResult rule: Contract.exhaust[case_product ReduceEffect.exhaust])
+  case Close_ReduceNoPayment
+  then show ?thesis using assms apply auto
+    by (cases "refundOne (accounts state)", auto)
+next
+  case (Close_ReduceWithPayment reducePayment)
+  then show ?thesis using assms apply auto
+(*Current place that's stuck.*)
+    by (cases "refundOne (accounts state)", auto)
+next
+  case (Pay_ReduceNoPayment accId payee token val cont)
+  then show ?thesis using assms apply auto
+    apply (cases "evalValue env state val \<le> 0", auto)
+     apply (metis PayNonPositive append_Nil2)
+    subgoal premises ps proof (cases "lookup (accId, token) (accounts state)")
+      case None
+      moreover have "(min 0 (evalValue env state val)) = 0" using ps(4) by auto
+      ultimately show ?thesis using ps apply auto
+        subgoal premises ps proof (cases "giveMoney payee token 0 (MList.delete (accId, token) (accounts state))")
+          case (Pair payment finalAccs)
+          moreover from ps have "(Contract.Pay accId payee token val continueContract, state, env,
+                     initialWarnings, initialPayments) \<rightarrow>
+                   (continueContract, state\<lparr>accounts := finalAccs\<rparr>, env,
+                    initialWarnings @ [ReducePartialPay accId payee token 0 (evalValue env state val)],
+                    initialPayments @ [])" using ps calculation by auto
+          ultimately show ?thesis using ps by (smt ReduceStepResult.inject State.simps(6) State.surjective old.prod.case)
+        qed
+        done
+    next
+      case (Some availableBal)
+      moreover have "availableBal \<le> evalValue env state val \<Longrightarrow> min availableBal (evalValue env state val) = availableBal" by simp
+      moreover have "\<not>(availableBal \<le> evalValue env state val) \<Longrightarrow> min availableBal (evalValue env state val) = (evalValue env state val)" by simp
+      ultimately show ?thesis using ps apply auto
+        apply (cases "availableBal \<le> evalValue env state val", auto)
+        subgoal premises ps proof (cases "giveMoney payee token availableBal (MList.delete (accId, token) (accounts state))")
+          case (Pair payment finalAccs)
+          then show ?thesis using ps apply auto
+            apply (cases "availableBal < (evalValue env state val)", auto)
+            subgoal premises ps proof -
+              from ps have "(Contract.Pay accId payee token val continueContract, state, env,
+                             initialWarnings, initialPayments) \<rightarrow>
+                           (continueContract, state\<lparr>accounts := finalAccs\<rparr>, env,
+                            initialWarnings @ [ReducePartialPay accId payee token availableBal (evalValue env state val)],
+                            initialPayments @ [])" by auto
+              then show ?thesis by meson
+            qed
+            subgoal premises ps proof -
+              from ps have "(Contract.Pay accId payee token val continueContract, state, env,
+                              initialWarnings, initialPayments) \<rightarrow>
+                             (continueContract, state\<lparr>accounts := finalAccs\<rparr>, env,
+                              initialWarnings @ [ReduceNoWarning], initialPayments @ [])" by auto
+              then show ?thesis by meson
+            qed
+            done
+        qed
+        subgoal premises ps proof (cases "giveMoney payee token (evalValue env state val) (MList.insert (accId, token) (availableBal - (evalValue env state val)) (accounts state))")
+          case (Pair payment finalAccs)
+          then show ?thesis using ps apply auto
+            subgoal premises ps proof -
+              from ps have "(Contract.Pay accId payee token val continueContract, state, env,
+                              initialWarnings, initialPayments) \<rightarrow>
+                             (continueContract, state\<lparr>accounts := finalAccs\<rparr>, env,
+                              initialWarnings @ [ReduceNoWarning], initialPayments @ [])" by auto
+              then show ?thesis by meson
+            qed
+            done
+        qed
+        done
+    qed
+    done
+next
+  case (Pay_ReduceWithPayment accId payee token val cont payment)
+  then show ?thesis using assms apply auto
+    apply (cases "evalValue env state val \<le> 0", auto)
+    subgoal premises ps proof (cases "lookup (accId, token) (accounts state)")
+      case None
+      moreover from ps have "min 0 (evalValue env state val) = 0" by simp
+      ultimately show ?thesis using ps apply auto
+        subgoal premises ps proof (cases "giveMoney payee token 0 (MList.delete (accId, token) (accounts state))")
+          case (Pair reduceEffect finalAccs)
+          moreover from ps calculation have "(Contract.Pay accId payee token val continueContract, state, env,
+                              initialWarnings, initialPayments) \<rightarrow>
+                             (continueContract, state\<lparr>accounts := finalAccs\<rparr>, env,
+                              initialWarnings @ [ReducePartialPay accId payee token 0 (evalValue env state val)],
+                              initialPayments @ [payment])" by auto
+          (*by auto before elimination rules*)
+          ultimately show ?thesis using ps by (auto, meson)
+        qed
+        done
+    next
+      case (Some bal)
+      then show ?thesis using ps apply auto
+        apply (cases "bal \<le> evalValue env state val", auto)
+        subgoal premises ps proof -
+          from ps have "min bal (evalValue env state val) = bal" by simp
+          then show ?thesis using ps apply auto
+            subgoal premises ps proof (cases "giveMoney payee token bal (MList.delete (accId, token) (accounts state))")
+              case (Pair reduceEffect finalAccs)
+              then show ?thesis using ps apply auto
+                apply (cases "bal < evalValue env state val", auto)
+                subgoal premises ps proof -
+                  from ps have "(Contract.Pay accId payee token val continueContract, state, env,
+                                initialWarnings, initialPayments) \<rightarrow>
+                               (continueContract, state\<lparr>accounts := finalAccs\<rparr>, env,
+                                initialWarnings @ [ReducePartialPay accId payee token bal (evalValue env state val)],
+                                initialPayments @ [payment])" by simp
+                  then show ?thesis by meson
+                qed
+                subgoal premises ps proof -
+                  from ps have "(Contract.Pay accId payee token val continueContract, state, env,
+                                initialWarnings, initialPayments) \<rightarrow>
+                               (continueContract, state\<lparr>accounts := finalAccs\<rparr>, env,
+                                initialWarnings @ [ReduceNoWarning], initialPayments @ [payment])" by simp
+                  then show ?thesis by meson
+                qed
+                done
+            qed
+            done
+        qed
+        subgoal premises ps proof -
+          from ps have "min bal (evalValue env state val) = evalValue env state val" by simp
+          then show ?thesis using ps apply auto
+            subgoal premises ps proof (cases "giveMoney payee token (evalValue env state val) (MList.insert (accId, token) (bal - (evalValue env state val)) (accounts state))")
+              case (Pair reduceEffect finalAccs)
+              moreover from ps calculation have "(Contract.Pay accId payee token val continueContract, state, env,
+                                  initialWarnings, initialPayments) \<rightarrow>
+                                 (continueContract, state\<lparr>accounts := finalAccs\<rparr>, env,
+                                  initialWarnings @ [ReduceNoWarning], initialPayments @ [payment])" by auto
+              (*used calculation by auto before elimination rules*)
+              then show ?thesis using ps by (auto, meson)
+            qed
+            done
+        qed
+        done
+    qed
+    done
+
+next
+  case (If_ReduceNoPayment x31 x32 x33)
+  then show ?thesis using assms apply auto
+     apply (metis IfTrue append_Nil2)
+    by (metis IfFalse append.right_neutral)
+next
+  case (If_ReduceWithPayment x31 x32 x33 x2)
+  then show ?thesis using assms by auto
+next
+  case (When_ReduceNoPayment x41 timeout x43)
+  then show ?thesis using assms apply auto
+    subgoal premises ps proof (cases "slotInterval env")
+      case (Pair ss es)
+      then show ?thesis using ps apply auto
+        apply (cases "es < timeout", auto)
+        apply (cases "timeout \<le> ss", auto)
+        by (smt WhenTimeout append_Nil2)
+    qed
+    done
+(*Removed LetC and UseC cases*)
+next
+  case (When_ReduceWithPayment x41 x42 x43 x2)
+  then show ?thesis using assms apply auto
+  by (smt ReduceStepResult.distinct(1) ReduceStepResult.distinct(3) ReduceStepResult.inject Pair_inject ReduceEffect.distinct(1) fixInterval.cases old.prod.case)
+next
+  case (Let_ReduceNoPayment vid x52 x53)
+  then show ?thesis using assms apply auto
+    apply (cases "lookup vid (boundValues state)", auto)
+     apply (metis LetNoShadow append_Nil2)
+    by (metis (no_types, lifting) ReduceStepResult.inject LetShadow State.unfold_congs(3) append_Nil2)
+next
+  case (Let_ReduceWithPayment vid x52 x53 x2)
+  then show ?thesis using assms apply auto
+    apply (cases "lookup vid (boundValues state)", auto)
+    by (meson ReduceStepResult.inject ReduceEffect.distinct(1))
+next
+  case (Assert_ReduceNoPayment x61 x62)
+  then show ?thesis using assms apply auto
+     apply (metis AssertTrue append.right_neutral)
+    by (metis AssertFalse append_Nil2)
+next
+  case (Assert_ReduceWithPayment x61 x62 x2)
+  then show ?thesis using assms by auto
+next
+qed
+
+lemma reduceStepIsSmallStepReductionNoPayment:
+assumes "reduceContractStep env state contract = Reduced warning ReduceNoPayment newState continueContract"
+shows "(contract, state, env, initialWarnings, initialPayments) \<rightarrow> (continueContract, newState, env, initialWarnings @ [warning], initialPayments)"
+proof (cases contract)
+  case Close
+  then show ?thesis using assms apply auto
+    by (cases "refundOne (accounts state)", auto)
+next
+  case (Pay accId payee token val cont)
+  then show ?thesis using assms apply auto
+    apply (cases "evalValue env state val \<le> 0", auto)
+    subgoal premises ps proof (cases "lookup (accId, token) (accounts state)")
+      case None
+      moreover have "(min 0 (evalValue env state val)) = 0" using ps by auto
+      ultimately show ?thesis using ps apply auto
+        subgoal premises ps proof (cases "giveMoney payee token 0 (MList.delete (accId, token) (accounts state))")
+          case (Pair payment finalAccs)
+          moreover from ps have "(Contract.Pay accId payee token val continueContract, state, env,
+                     initialWarnings, initialPayments) \<rightarrow>
+                   (continueContract, state\<lparr>accounts := finalAccs\<rparr>, env,
+                    initialWarnings @ [ReducePartialPay accId payee token 0 (evalValue env state val)],
+                    initialPayments @ [])" using ps calculation by auto
+          ultimately show ?thesis using ps by simp
+        qed
+        done
+    next
+      case (Some availableBal)
+      moreover have "availableBal \<le> evalValue env state val \<Longrightarrow> min availableBal (evalValue env state val) = availableBal" by simp
+      moreover have "\<not>(availableBal \<le> evalValue env state val) \<Longrightarrow> min availableBal (evalValue env state val) = (evalValue env state val)" by simp
+      ultimately show ?thesis using ps apply auto
+        apply (cases "availableBal \<le> evalValue env state val", auto)
+        subgoal premises ps proof (cases "giveMoney payee token availableBal (MList.delete (accId, token) (accounts state))")
+          case (Pair payment finalAccs)
+          then show ?thesis using ps by (cases "availableBal < (evalValue env state val)", auto)
+        qed
+        subgoal premises ps proof (cases "giveMoney payee token (evalValue env state val) (MList.insert (accId, token) (availableBal - (evalValue env state val)) (accounts state))")
+          case (Pair payment finalAccs)
+          then show ?thesis using ps by auto
+        qed
+        done
+    qed
+    done
+next
+  case (If x31 x32 x33)
+  then show ?thesis using assms by auto
+next
+  case (When x41 timeout x43)
+  then show ?thesis using assms apply auto
+    subgoal premises ps proof (cases "slotInterval env")
+      case (Pair ss es)
+      then show ?thesis using ps apply auto
+        apply (cases "es < timeout", auto)
+        by (cases "timeout \<le> ss", auto)
+    qed
+    done
+next
+  case (Let vid x52 x53)
+  then show ?thesis using assms apply auto
+    apply (cases "lookup vid (boundValues state)", auto)
+    by (metis (no_types, lifting) ReduceStepResult.inject LetShadow State.unfold_congs(3))
+next
+  case (Assert x61 x62)
+  then show ?thesis using assms by auto
+qed
+
+lemma reduceStepIsSmallStepReductionWithPayment:
+assumes "reduceContractStep env state contract = Reduced warning (ReduceWithPayment payment) newState continueContract"
+shows "(contract, state, env, initialWarnings, initialPayments) \<rightarrow> (continueContract, newState, env, initialWarnings @ [warning], initialPayments @ [payment])"
+proof (cases contract)
+  case (Close)
+  then show ?thesis using assms by (cases "refundOne (accounts state)", auto)
+next
+  case (Pay accId payee token val cont)
+  then show ?thesis using assms apply auto
+    apply (cases "evalValue env state val \<le> 0", auto)
+    subgoal premises ps proof (cases "lookup (accId, token) (accounts state)")
+      case None
+      moreover from ps have "min 0 (evalValue env state val) = 0" by simp
+      ultimately show ?thesis using ps apply auto
+        subgoal premises ps proof (cases "giveMoney payee token 0 (MList.delete (accId, token) (accounts state))")
+          case (Pair reduceEffect finalAccs)
+          moreover from ps calculation have "(Contract.Pay accId payee token val continueContract, state, env,
+                              initialWarnings, initialPayments) \<rightarrow>
+                             (continueContract, state\<lparr>accounts := finalAccs\<rparr>, env,
+                              initialWarnings @ [ReducePartialPay accId payee token 0 (evalValue env state val)],
+                              initialPayments @ [payment])" by auto
+          ultimately show ?thesis using ps by auto
+        qed
+        done
+    next
+      case (Some bal)
+      then show ?thesis using ps apply auto
+        apply (cases "bal \<le> evalValue env state val", auto)
+        subgoal premises ps proof -
+          from ps have "min bal (evalValue env state val) = bal" by simp
+          then show ?thesis using ps apply auto
+            subgoal premises ps proof (cases "giveMoney payee token bal (MList.delete (accId, token) (accounts state))")
+              case (Pair reduceEffect finalAccs)
+              then show ?thesis using ps by (cases "bal < evalValue env state val", auto)
+            qed
+            done
+        qed
+        subgoal premises ps proof -
+          from ps have "min bal (evalValue env state val) = evalValue env state val" by simp
+          then show ?thesis using ps apply auto
+            subgoal premises ps proof (cases "giveMoney payee token (evalValue env state val) (MList.insert (accId, token) (bal - (evalValue env state val)) (accounts state))")
+              case (Pair reduceEffect finalAccs)
+              moreover from ps calculation have "(Contract.Pay accId payee token val continueContract, state, env,
+                                  initialWarnings, initialPayments) \<rightarrow>
+                                 (continueContract, state\<lparr>accounts := finalAccs\<rparr>, env,
+                                  initialWarnings @ [ReduceNoWarning], initialPayments @ [payment])" by auto
+              then show ?thesis using ps by (auto, meson)
+            qed
+            done
+        qed
+        done
+    qed
+    done
+next
+  case (If x31 x32 x33)
+  then show ?thesis using assms by auto
+next
+  case (When x41 x42 x43)
+  then show ?thesis using assms apply auto
+  by (smt ReduceStepResult.distinct(1) ReduceStepResult.distinct(3) ReduceStepResult.inject Pair_inject ReduceEffect.distinct(1) fixInterval.cases old.prod.case)
+next
+  case (Let vid x52 x53)
+  then show ?thesis using assms apply auto
+    apply (cases "lookup vid (boundValues state)", auto)
+    by (meson ReduceStepResult.inject ReduceEffect.distinct(1))
+next
+  case (Assert x61 x62)
+  then show ?thesis using assms by auto
+qed
+
+(*BEGIN proof Small Step in Marlowe implies that there is a Reduced Step*)
+
+lemma smallStepReductionAddsOneWarning:
+assumes "cs = (contract, state, env, initialWarnings, initialPayments) \<and>
+    cs' = (continueContract, newState, newEnv, newWarnings, newPayments) \<and>
+    cs \<rightarrow> cs'"
+shows "\<exists>newWarning . newWarnings = initialWarnings @ [newWarning]"
+proof (cases contract)
+  case Close
+  then show ?thesis using assms by auto
+next
+  case (Pay accId payee token val cont)
+  then show ?thesis using assms by auto
+next
+  case (If x31 x32 x33)
+  then show ?thesis using assms by auto
+next
+  case (When cases timeout cont)
+  then show ?thesis using assms by auto
+next
+  case (Let x51 x52 x53)
+  then show ?thesis using assms by auto
+next
+  case (Assert x61 x62)
+  then show ?thesis using assms by auto
+qed
+
+lemma smallStepReductionImpReduceStep:
+assumes "cs = (contract, state, env, initialWarnings, initialPayments) \<and>
+    cs' = (continueContract, newState, newEnv, initialWarnings @ [warning], newPayments) \<and>
+    cs \<rightarrow> cs'"
+shows "\<exists> paymentReduceResult . reduceContractStep env state contract = Reduced warning paymentReduceResult newState continueContract"
+proof (cases contract)
+  case Close
+  then show ?thesis using assms by auto
+next
+  case (Pay accId payee token val cont)
+  then show ?thesis using assms by (auto simp add: min.strict_order_iff min.absorb_iff2)
+next
+  case (If x31 x32 x33)
+  then show ?thesis using assms by auto
+next
+  case (When cases timeout cont)
+  then show ?thesis using assms by auto
+next
+  case (Let x51 x52 x53)
+  then show ?thesis using assms apply auto
+    by metis
+next
+  case (Assert x61 x62)
+  then show ?thesis using assms by auto
+qed
+
+lemma smallStepReductionGivesOnePaymentMax:
+assumes "cs = (contract, state, env, initialWarnings, initialPayments) \<and>
+    cs' = (continueContract, newState, newEnv, initialWarnings @ [warning], newPayments) \<and>
+    cs \<rightarrow> cs'"
+shows "newPayments = initialPayments \<or> (\<exists>newPayment . newPayments = initialPayments @ [newPayment])"
+proof (cases contract)
+  case Close
+  then show ?thesis using assms by auto
+next
+  case (Pay x21 x22 x23 x24 x25)
+  then show ?thesis using assms by auto
+next
+  case (If x31 x32 x33)
+  then show ?thesis using assms by auto
+next
+  case (When x41 x42 x43)
+  then show ?thesis using assms by auto
+next
+  case (Let x51 x52 x53)
+  then show ?thesis using assms by auto
+next
+  case (Assert x61 x62)
+  then show ?thesis using assms by auto
+qed
+
+lemma smallStepReductionImpReduceStepNoPayment:
+assumes "cs = (contract, state, env, initialWarnings, initialPayments) \<and>
+    cs' = (continueContract, newState, newEnv, initialWarnings @ [warning], initialPayments) \<and>
+    cs \<rightarrow> cs'"
+shows "reduceContractStep env state contract = Reduced warning ReduceNoPayment newState continueContract"
+proof (cases contract)
+  case Close
+  then show ?thesis using assms by auto
+next
+  case (Pay accId payee token val cont)
+  then show ?thesis using assms by (auto simp add: min.strict_order_iff min.absorb_iff2)
+next
+  case (If x31 x32 x33)
+  then show ?thesis using assms by auto
+next
+  case (When cases timeout cont)
+  then show ?thesis using assms by auto
+next
+  case (Let x51 x52 x53)
+  then show ?thesis using assms apply auto
+    by metis
+next
+  case (Assert x61 x62)
+  then show ?thesis using assms by auto
+qed
+
+lemma smallStepReductionImpReduceStepWithPayment:
+assumes "cs = (contract, state, env, initialWarnings, initialPayments) \<and>
+    cs' = (continueContract, newState, newEnv, initialWarnings @ [warning], initialPayments @ [newPayment]) \<and>
+    cs \<rightarrow> cs'"
+shows "reduceContractStep env state contract = Reduced warning (ReduceWithPayment newPayment) newState continueContract"
+proof (cases contract)
+  case Close
+  then show ?thesis using assms by auto
+next
+  case (Pay accId payee token val cont)
+  then show ?thesis using assms by (auto simp add: min.strict_order_iff min.absorb_iff2)
+next
+  case (If x31 x32 x33)
+  then show ?thesis using assms by auto
+next
+  case (When cases timeout cont)
+  then show ?thesis using assms by auto
+next
+  case (Let x51 x52 x53)
+  then show ?thesis using assms by auto
+next
+  case (Assert x61 x62)
+  then show ?thesis using assms by auto
+qed
+
+end
